---
id: "714262"
title: "String Mirror"
slug: "string-mirror--170647"
difficulty: "Easy"
companyTags: []
tags: ["Strings", "Mathematical", "Data Structures", "Algorithms"]
---

Here is the Markdown blog post for the "String Mirror" problem:

**String Mirror**
================

### Summary

The String Mirror problem involves creating a new string that is the mirror reflection of the input string. The task is to create an algorithm that takes a given string as input and returns the mirrored version of the string. This problem requires understanding of basic string manipulation techniques.

### Detailed Explanation

To solve this problem, we can use a simple approach where we iterate over the input string from both ends (start and end) and construct the mirrored string.

Here's a step-by-step breakdown of the solution:

1. Initialize an empty string `mirrored_str` to store the result.
2. Iterate over the input string `str` from both ends (start and end).
3. For each character at position `i`, add the corresponding character at position `n-i-1` (where `n` is the length of the input string) to `mirrored_str`. This ensures that characters are mirrored correctly.
4. Continue this process until you reach the middle of the input string (or the beginning of the end, depending on whether the input string has an even or odd length).
5. Return the constructed `mirrored_str` as the result.

Time complexity: O(n), where n is the length of the input string.
Space complexity: O(n), since we need to store the mirrored string.

### Optimized Solutions

#### Java
```java
public String stringMirror(String str) {
    StringBuilder mirroredStr = new StringBuilder();
    int n = str.length();
    for (int i = 0; i < n / 2; i++) {
        mirroredStr.append(str.charAt(n - i - 1));
        if (i != n / 2) {
            mirroredStr.append(str.charAt(i));
        }
    }
    return mirroredStr.toString();
}
```

#### Python
```python
def string_mirror(s):
    mirrored_str = ""
    n = len(s)
    for i in range(n // 2):
        mirrored_str += s[n - i - 1]
        if i != n // 2:
            mirrored_str += s[i]
    return mirrored_str
```

#### C++
```cpp
string stringMirror(string str) {
    string mirroredStr = "";
    int n = str.length();
    for (int i = 0; i < n / 2; i++) {
        mirroredStr += str.substr(n - i - 1, 1);
        if (i != n / 2) {
            mirroredStr += str.substr(i, 1);
        }
    }
    return mirroredStr;
}
```

#### JavaScript
```javascript
function stringMirror(s) {
    let mirroredStr = "";
    const n = s.length;
    for (let i = 0; i < Math.floor(n / 2); i++) {
        mirroredStr += s[n - i - 1];
        if (i !== Math.floor(n / 2)) {
            mirroredStr += s[i];
        }
    }
    return mirroredStr;
}
```

Note that these optimized solutions use the same approach as described in the detailed explanation, with slight variations to suit each programming language.